src/program_proof/ctrexample/interface.v
@@ -4,6 +4,8 @@ From Perennial.program_proof Require Import proof_prelude.
 From iris.algebra Require Export mono_nat.
 From Perennial.program_proof.memkv Require Import rpc_spec.
 From Perennial.program_proof Require Import marshal_proof.
+From Perennial.program_proof.memkv Require Import rpc_proof.
+From Perennial.base_logic Require Import lib.ghost_map lib.saved_spec.
 
 Section interface.
 
@@ -12,12 +14,18 @@ Context `{!inG Σ mono_natUR}.
 Definition counter_lb γ (x:nat) : iProp Σ := own γ (◯MN x).
 Definition counter_own γ (x:nat) : iProp Σ := own γ (●MN x).
 
+Context `{!rpcregG Σ}.
 Context `{HPRE: !gooseGlobalGS Σ}.
-Definition FAISpec γ (reqData:list u8) (Φ:list u8 → iProp Σ) : iProp Σ :=
-  □(
+
+Program Definition FAISpec (γ:gname) : savedSpecO Σ (list u8) (list u8) :=
+  λ reqData, λne (Φ : list u8 -d> iPropO Σ),
+  (□(
       ∀ (x:nat), counter_own γ x ={⊤}=∗ counter_own γ (x + 1) ∗
                                     (∀ l, ⌜has_encoding l [EncUInt64 x]⌝ -∗ Φ l)
-    )
+    ))%I
 .
+Next Obligation.
+  solve_proper.
+Defined.
 
 End interface.
